ulib/experimental/Steel.ArrayStruct.fst
@@ -1,0 +1,81 @@
+(*
+   Copyright 2020 Microsoft Research
+
+   Licensed under the Apache License, Version 2.0 (the "License");
+   you may not use this file except in compliance with the License.
+   You may obtain a copy of the License at
+
+       http://www.apache.org/licenses/LICENSE-2.0
+
+   Unless required by applicable law or agreed to in writing, software
+   distributed under the License is distributed on an "AS IS" BASIS,
+   WITHOUT WARRANTIES OR CONDITIONS OF ANY KIND, either express or implied.
+   See the License for the specific language governing permissions and
+   limitations under the License.
+*)
+
+module Steel.ArrayStruct
+
+module SizeT = Steel.SizeT
+module Map = FStar.Map
+
+
+open FStar.FunctionalExtensionality
+open Steel.PCM
+module PCMBase = Steel.PCM.Base
+
+open Steel.Effect.Fake
+open Steel.Memory
+
+let extract_update: unit -> Tot unit = (fun () -> ())
+let extract_get: unit -> Tot unit = (fun () -> ())
+let extract_explode: unit -> Tot unit = (fun () -> ())
+let extract_recombine: unit -> Tot unit = (fun () -> ())
+let op_String_Access : unit -> Tot unit = (fun () -> ())
+let generic_index: unit -> Tot unit = (fun () -> ())
+
+assume val witness_h_exists (#a:Type) (#p:a -> slprop) (_:unit)
+  : SteelT (Ghost.erased a) (h_exists p) (fun x -> p x)
+
+assume val h_assert (p:slprop)
+  : SteelT unit p (fun _ -> p)
+
+assume val intro_h_exists (#a:Type) (x:a) (p:(a -> slprop))
+  : SteelT unit (p x) (fun _ -> h_exists p)
+
+assume val intro_h_exists_erased (#a:Type) (x:Ghost.erased a) (p:(a -> slprop))
+  : SteelT unit (p x) (fun _ -> h_exists p)
+
+assume val reveal_val (#a:Type u#1) (#pcm:pcm a) (r:ref a pcm)
+  : Steel (Ghost.erased a) (ptr r) (fun v -> pts_to r v) (fun _ -> True) (fun h0 v h1 ->
+    Steel.Memory.intro_h_exists (Ghost.reveal v) (pts_to r) h1;
+    sel r h0 == sel r h1 /\ sel r h1 == Ghost.reveal v
+  )
+
+#set-options "--fuel 1 --ifuel 0 --print_implicits"
+
+let update_x (r: ref (option u32_pair) u32_pair_pcm) (new_val: UInt32.t)
+    : Steel unit (href r) (fun _ -> href r)
+    (fun h0 -> if Some? (sel r h0) then True else False) (fun h0 _ h1 ->
+     Some? (sel r h1) /\ Some? (sel r h0) /\
+     Some?.v (sel r h1) == { Some?.v (sel r h0) with x = new_val }
+    )
+  =
+  let old_pair_ghost : Ghost.erased (option u32_pair) =
+    reveal_val r
+  in
+  let old_pair = read r old_pair_ghost in
+  assert(FStar.PCM.compatible u32_pair_pcm (Ghost.reveal old_pair_ghost) old_pair);
+  compatible_elim u32_pair_pcm (Ghost.reveal old_pair_ghost) (old_pair)
+    (Ghost.reveal old_pair_ghost == old_pair) (fun frame ->
+      assert(Some? old_pair_ghost);
+      assert(None? frame);
+      assert(Some? old_pair);
+      assert(Some?.v old_pair_ghost == Some?.v old_pair);
+      admit()
+    );
+  let new_pair = (Some ({Some?.v old_pair with x = new_val })) in
+  //write r old_pair new_pair;
+  //intro_h_exists new_pair (pts_to r);
+  intro_h_exists_erased old_pair_ghost (pts_to r);
+  admit()
